%\begin{preamble}
\documentclass{article}
\usepackage{amsthm}
\usepackage{amsmath}
\usepackage{mathtools}
\usepackage{amssymb}
\usepackage{example}
\usepackage{qtree}
\usepackage{stmaryrd}
\newcommand{\sv}[1]{\ensuremath{\llbracket #1 \rrbracket}}
\newcommand{\AB}[1]{\ensuremath{\langle #1 \rangle}}
\newcommand{\bsf}[1]{\textsf{\bfseries #1}}
\newcommand{\ceq}{\ensuremath{\coloneqq}}
\newcommand{\ra}{\ensuremath{\rightarrow}}
\usepackage[margin=1in]{geometry}
\usepackage[normalem]{ulem}
\usepackage{hyperref}
%\end{preamble}
\begin{document}

\noindent\textbf{\Large Homework for Friday October 10, 2014}


\section{More practice with $\lambda$s}

\renewcommand{\arraystretch}{1.3}
\[\begin{array}{r@{}ll}
	(\lambda m.\lambda n.m(\lambda f.n(\lambda x.f(x))))(\lambda k.k(\text{left}'))(\lambda k.k(x)) &{}= (\lambda n.(\lambda k.k(\text{left}'))(\lambda f.n(\lambda x.f(x))))(\lambda k.k(x)) & \beta%
	\\
	&{}= (\lambda k.k(\text{left}'))(\lambda f.(\lambda k.k(x))(\lambda x.f(x))) & \beta%
	\\
	&{}= (\lambda f.(\lambda k.k(x))(\lambda x.f(x)))(\text{left}') & \beta%
	\\
	&{}= (\lambda k.k(x))(\lambda x.\text{left}'(x)) & \beta%
	\\
	&{}= (\lambda x.\text{left}'(x))(x) & \beta%
	\\
	&{}= \text{left}'(x) & \beta%
\end{array}\]


\section{Relative clauses}

\begin{itemize}	
	\item \textsf{the cat Uni likes hates her}:
	\begin{figure}[!ht]
	\[\begin{array}{c}
		\begin{array}{c}
			\textsf{\Tree [.A [.B the [.C cat [.D 1 [.E Uni [.F likes $t_1$ ] ] ] ] ] !\qsetw{10em} [.G hates her$_1$ ] ]}%
		\end{array}
		\\\\
		\renewcommand{\arraystretch}{1.3}
		\begin{array}{r@{}ll}
			\sv{\textsf{A}}^g &{}= \sv{\textsf{G}}^g(\sv{\textsf{B}}^g) & \bsf{FA}
			\\
			&{}= \sv{\textsf{G}}^g(\sv{\textsf{the}}^g(\sv{\textsf{C}}^g)) & \bsf{FA}
			\\
			&{}= \sv{\textsf{G}}^g(\sv{\textsf{the}}^g(\lambda x.\sv{\textsf{cat}}^g(x)=\sv{\textsf{D}}^g(x)=1)) & \bsf{PM}%
			\\
			&{}= \sv{\textsf{G}}^g(\sv{\textsf{the}}^g(\lambda x.\sv{\textsf{cat}}^g(x)=(\lambda y.\sv{\textsf{E}}^{g[y/1]})(x)=1)) & \bsf{PA}%
			\\
			&{}= \sv{\textsf{G}}^g(\sv{\textsf{the}}^g(\lambda x.\sv{\textsf{cat}}^g(x)=\sv{\textsf{E}}^{g[x/1]}=1)) & \beta%
			\\
			&{}= \sv{\textsf{G}}^g(\sv{\textsf{the}}^g(\lambda x.\sv{\textsf{cat}}^g(x)=\sv{\textsf{F}}^{g[x/1]}(\sv{\textsf{Uni}}^{g[x/1]})=1)) & \bsf{FA}%
			\\
			&{}= \sv{\textsf{G}}^g(\sv{\textsf{the}}^g(\lambda x.\sv{\textsf{cat}}^g(x)=\sv{\textsf{likes}}^{g[x/1]}(\sv{t_1}^{g[x/1]})(\sv{\textsf{Uni}}^{g[x/1]})=1)) & \bsf{FA}%
			\\
			&{}= \sv{\textsf{hates}}^g(\sv{\textsf{her}_1}^g)(\sv{\textsf{the}}^g(\lambda x.\sv{\textsf{cat}}^g(x)=\sv{\textsf{likes}}^{g[x/1]}(\sv{t_1}^{g[x/1]})(\sv{\textsf{Uni}}^{g[x/1]})=1)) & \bsf{FA}%
			\\
			&{}= \text{hates}'(\sv{\textsf{her}_1}^g)(\sv{\textsf{the}}^g(\lambda x.\,\text{cat}'(x)=\text{likes}'(\sv{t_1}^{g[x/1]})(\text{u})=1)) & \text{Lexicon}%
			\\
			&{}= \text{hates}'(g(1))(\sv{\textsf{the}}^g(\lambda x.\,\text{cat}'(x)=\text{likes}'(x)(\text{u})=1)) & \text{Variables}%
			\\
			&{}= \text{hates}'(g(1))((\lambda P.\iota x.P(x))(\lambda x.\,\text{cat}'(x)=\text{likes}'(x)(\text{u})=1)) & \text{Lexicon}%
			\\
			&{}= \text{hates}'(g(1))(\iota x.\,\text{cat}'(x)=\text{likes}'(x)(\text{u})=1) & \beta%
		\end{array}
	\end{array}\]
%	\caption{In prose: true iff the $x$ such that $x$ is a cat and Uni likes $x$ hates $g(1)$.}
	\label{fig1}
	\end{figure}
	
%	\item Here's a possible tree for the bigger relative clause in the DP \textsf{the man who saw the cat who meowed}. %
	
	\[\begin{array}{c}
		\textsf{$\begin{array}{c}
			\Tree [.A 1 [.B $t_1$ [.C saw [.D the [.E cat [.F who [.G 1 [.H $t_1$ meowed ] ] ] ] ] ] ] ]%
		\end{array}$}
		\\\\
		\begin{array}{r@{}ll}
			\sv{\textsf{A}}^g &{}= \lambda x.\sv{\textsf{B}}^{g[x/1]} & \bsf{PA}
			\\
			&{}= \lambda x.\sv{\textsf{C}}^{g[x/1]}(\sv{t_1}^{g[x/1]}) & \bsf{FA}
			\\
			&{}= \lambda x.\sv{\textsf{C}}^{g[x/1]}(x) & \text{Variables}
			\\
			&{}= \lambda x.\sv{\textsf{saw}}^{g[x/1]}(\sv{\textsf{D}}^{g[x/1]})(x) & \bsf{FA}%
			\\
			&{}= \lambda x.\,\text{saw}'(\sv{\textsf{D}}^{g[x/1]})(x) & \text{Lexicon}%
			\\
			&{}= \lambda x.\,\text{saw}'(\sv{\textsf{the}}^{g[x/1]}(\sv{\textsf{E}}^{g[x/1]}))(x) & \bsf{FA}%
			\\
			&{}= \lambda x.\,\text{saw}'(\sv{\textsf{the}}^{g[x/1]}(\lambda y.\sv{\textsf{cat}}^{g[x/1]}(y) = \sv{\textsf{F}}^{g[x/1]}(y)=1))(x) & \bsf{PM}%
			\\
			&{}= \lambda x.\,\text{saw}'(\sv{\textsf{the}}^{g[x/1]}(\lambda y.\,\text{cat}'(y) = \sv{\textsf{F}}^{g[x/1]}(y)=1))(x) & \text{Lexicon}%
			\\
			&{}= \lambda x.\,\text{saw}'(\sv{\textsf{the}}^{g[x/1]}(\lambda y.\,\text{cat}'(y) = \sv{\textsf{who}}^{g[x/1]}(\sv{\textsf{G}}^{g[x/1]})(y)=1))(x) & \bsf{FA}%
			\\
			&{}= \lambda x.\,\text{saw}'(\sv{\textsf{the}}^{g[x/1]}(\lambda y.\,\text{cat}'(y) = (\lambda P.P)(\sv{\textsf{G}}^{g[x/1]})(y)=1))(x) & \text{Lexicon}%
			\\
			&{}= \lambda x.\,\text{saw}'(\sv{\textsf{the}}^{g[x/1]}(\lambda y.\,\text{cat}'(y) = (\sv{\textsf{G}}^{g[x/1]})(y)=1))(x) & \beta%
			\\
			&{}= \lambda x.\,\text{saw}'(\sv{\textsf{the}}^{g[x/1]}(\lambda y.\,\text{cat}'(y) = (\lambda y.\sv{\textsf{H}}^{g[x/1][y/1]})(y)=1))(x) & \bsf{PA}%
			\\
			&{}= \lambda x.\,\text{saw}'(\sv{\textsf{the}}^{g[x/1]}(\lambda y.\,\text{cat}'(y) = \sv{\textsf{H}}^{g[x/1][y/1]}=1))(x) & \beta%
			\\
			&{}= \lambda x.\,\text{saw}'(\sv{\textsf{the}}^{g[x/1]}(\lambda y.\,\text{cat}'(y) = \sv{\textsf{meowed}}^{g[x/1][y/1]}(\sv{t_1}^{g[x/1][y/1]})=1))(x) & \bsf{FA}%
			\\
			&{}= \lambda x.\,\text{saw}'(\sv{\textsf{the}}^{g[x/1]}(\lambda y.\,\text{cat}'(y) = \text{meowed}'(\sv{t_1}^{g[x/1][y/1]})=1))(x) & \text{Lexicon}%
			\\
			&{}= \lambda x.\,\text{saw}'(\sv{\textsf{the}}^{g[x/1]}(\lambda y.\,\text{cat}'(y) = \text{meowed}'(y)=1))(x) & \text{Variables}%
			\\
			&{}= \lambda x.\,\text{saw}'((\lambda P.\iota y.P(y))(\lambda y.\,\text{cat}'(y) = \text{meowed}'(y)=1))(x) & \text{Lexicon}%
			\\
			&{}= \lambda x.\,\text{saw}'(\iota y.(\lambda y.\,\text{cat}'(y) = \text{meowed}'(y)=1)(y))(x) & \beta%
			\\
			&{}= \lambda x.\,\text{saw}'(\iota y.\,\text{cat}'(y) = \text{meowed}'(y)=1)(x) & \beta%
		\end{array}
	\end{array}\]
	\begin{itemize}
		\item[$\rhd$] We can sum up the state of affairs as follows: an abstraction index binds a pronoun/trace iff the number on the abstraction index is the same as the number on the pronoun/trace, the abstraction index c-commands the co-indexed pronoun/trace, and no other c-commanding, co-indexed abstraction index intervenes between the abstraction index and the pronoun/trace. Thus, \textsf{her}$_1$ is not bound in the first tree (since it is co-indexed but not c-commanded by the abstraction index), and the abstraction indices in the second tree bind the nearest traces. %
	\end{itemize}
	
\end{itemize}


\section{Quantifiers}

\begin{itemize}
	\item Meanings for quantificational DPs:%
	\begin{enumerate}
		\item $\sv{\textsf{not every phonologist}}^g = \lambda P.\,\text{phonologist}' \nsubseteq P$%
		
		\item $\sv{\textsf{three out of four dentists}}^g = \lambda P.\frac{|\text{dentist}' \cap P|}{|\text{dentist}'|} \geq \frac{3}{4}$%
		\begin{itemize}
			\item[$\rhd$] Note: we tend to hear sentences like \textsf{three out of four dentists agree} as entailing that \emph{no more than} three out of four agree. This is plausibly an implicature. Suppose I say \textsf{if three out of four dentists agree, this toothbrush gets approved}. Surely if four out of four approve, the toothbrush still gets approved.%
		\end{itemize}
		
		\item $\sv{\textsf{every linguist except John}}^g = \lambda P.\,(\text{linguist}' - \{\text{j}\}) \subseteq P\text{, and }\text{j} \notin P$%
		\begin{itemize}
			\item[$\rhd$] Note: this construction seems to \textbf{presuppose} that John is a linguist. If you like, you can write that into the meaning in terms of a definedness condition. Notice also that the second condition ($\{\text{j}\} \notin P$) is crucial. Without it, we do not end up entailing that John isn't among the people of whom $P$ holds. Do you see why?%
		\end{itemize}
		
		\item $\sv{\textsf{at least four but no more than ten hotels}}^g = \lambda P.\, 4 \leq |\text{hotel}' \cap P| \leq 10$%
		
		\item $\sv{\textsf{more than ten or fewer than five semanticists}}^g = \lambda P.\,|\text{sems}' \cap P| > 10\text{, or }|\text{sems}' \cap P| < 5$%		
	\end{enumerate}
	
	\item \textsf{the dog every linguist knows skijors}:%
	\[\begin{array}{c}
		\begin{array}{c}
			\textsf{\Tree [.\textsf{A} [.\textsf{B} the [.\textsf{C} dog [.\textsf{D} 8 !\qsetw{-5em} [.\textsf{E} {every linguist} [.\textsf{G} knows $t_8$ ] ] ] ] ] !\qsetw{10em} skijors ]}%
		\end{array}
		\\\\
		\begin{array}{r@{}ll}
			\sv{\textsf{A}}^g &{}= \sv{\textsf{skijors}}^g(\sv{\textsf{B}}^g) & \bsf{FA}
			\\
			&{}= \text{skijors}'(\sv{\textsf{B}}^g) & \text{Lexicon}
			\\
			&{}= \text{skijors}'(\sv{\textsf{the}}^g(\sv{\textsf{C}}^g)) & \bsf{FA}
			\\
			&{}= \text{skijors}'(\sv{\textsf{the}}^g(\lambda x.\sv{\textsf{dog}}^g(x) = \sv{\textsf{D}}^g(x) = 1)) & \bsf{PM}%
			\\
			&{}= \text{skijors}'(\sv{\textsf{the}}^g(\lambda x.\,\text{dog}'(x) = \sv{\textsf{D}}^g(x) = 1)) & \text{Lexicon}%
			\\
			&{}= \text{skijors}'(\sv{\textsf{the}}^g(\lambda x.\,\text{dog}'(x) = (\lambda x.\sv{\textsf{E}}^{g[x/8]})(x) = 1)) & \bsf{PA}%
			\\
			&{}= \text{skijors}'(\sv{\textsf{the}}^g(\lambda x.\,\text{dog}'(x) = \sv{\textsf{E}}^{g[x/8]} = 1)) & \beta%
			\\
			&{}= \text{skijors}'(\sv{\textsf{the}}^g(\lambda x.\,\text{dog}'(x) = \sv{\textsf{every linguist}}^{g[x/8]}(\sv{\textsf{G}}^{g[x/8]}) = 1)) & \bsf{FA}%
			\\
			&{}= \text{skijors}'(\sv{\textsf{the}}^g(\lambda x.\,\text{dog}'(x) = \sv{\textsf{every linguist}}^{g[x/8]}(\sv{\textsf{knows}}^{g[x/8]}(\sv{t_8}^{g[x/8]})) = 1)) & \bsf{FA}%
			\\
			&{}= \text{skijors}'(\sv{\textsf{the}}^g(\lambda x.\,\text{dog}'(x) = \sv{\textsf{every linguist}}^{g[x/8]}(\text{knows}'(\sv{t_8}^{g[x/8]})) = 1)) & \text{Lexicon}%
			\\
			&{}= \text{skijors}'(\sv{\textsf{the}}^g(\lambda x.\,\text{dog}'(x) = \sv{\textsf{every linguist}}^{g[x/8]}(\text{knows}'(x)) = 1)) & \text{Variables}%
			\\
			&{}= \text{skijors}'(\sv{\textsf{the}}^g(\lambda x.\,\text{dog}'(x) = (\lambda P.\,\text{ling}' \subseteq \{y : P(y)\})(\text{knows}'(x)) = 1)) & \text{Lexicon}%
			\\
			&{}= \text{skijors}'(\sv{\textsf{the}}^g(\lambda x.\,\text{dog}'(x) = \text{ling}' \subseteq \{y : \text{knows}'(x)(y)\} = 1)) & \beta%
			\\
			&{}= \text{skijors}'((\lambda P.\iota x.P(x))(\lambda x.\,\text{dog}'(x) = \text{ling}' \subseteq \{y : \text{knows}'(x)(y)\} = 1)) & \text{Lexicon}%
			\\
			&{}= \text{skijors}'(\iota x.(\lambda x.\,\text{dog}'(x) = \text{ling}' \subseteq \{y : \text{knows}'(x)(y)\} = 1)(x)) & \beta%
			\\
			&{}= \text{skijors}'(\iota x.\,\text{dog}'(x) = \text{ling}' \subseteq \{y : \text{knows}'(x)(y)\} = 1) & \beta%
		\end{array}
	\end{array}\]
	
	\item Type \AB{\AB{e,t},t} meanings for \textsf{New Jersey} and \textsf{the Queen of England}:%
	\begin{enumerate}
		\item $\lambda P.P(\text{nj})$
		\item $\lambda P.P(\text{qoe})$
	\end{enumerate}
	
%	\item What does your entry predict about the truth of \textsf{every unicorn came, and no unicorn came} in a world (like ours?) where unicorns fail to exist, i.e.~where $\sv{\textsf{unicorn}}^g = \emptyset$. What do you think of that?%
	
%	\item We saw in class that there was no way to compose a transitive verb (type \AB{e,\AB{e,t}}) with a quantificational DP (type \AB{\AB{e,t},t}). Here is one possible (though partial) fix. Assume the following silent morheme is freely available:  %
%	\[\sv{\textsf{BLA}_\emptyset}^g \ceq \lambda R_{\AB{e,\AB{e,t}}}.\lambda {\cal Q}_{\AB{\AB{e,t},t}}.\lambda x_e.{\cal Q}(\lambda y.R(y)(x))\]%
		\item Using \textsf{BLA}$_\emptyset$ to derive a meaning for the ambiguous sentence \textsf{somebody likes everybody} without QR. This is the surface-scope interpretation. \textsf{BLA}$_\emptyset$ by itself (and without QR) doesn't give us a way to derive the inverse-scope interpretation: %
		\[\begin{array}{c}
			\textsf{\Tree [.A somebody [.B [.C BLA$_\emptyset$ likes ] everybody ] ]}
			\\\\
			\begin{array}{r@{}ll}
				\sv{\textsf{A}}^g &{}= \sv{\textsf{somebody}}^g(\sv{\textsf{B}}^g) & \bsf{FA}%
				\\
				&{}= \sv{\textsf{somebody}}^g(\sv{\textsf{C}}^g(\sv{\textsf{everybody}}^g)) & \bsf{FA}%
				\\
				&{}= \sv{\textsf{somebody}}^g(\sv{\textsf{BLA}_\emptyset}^g(\sv{\textsf{likes}}^g)(\sv{\textsf{everybody}}^g)) & \bsf{FA}%
				\\
				&{}= \sv{\textsf{somebody}}^g((\lambda R.\lambda {\cal Q}.\lambda x.{\cal Q}(\lambda y.R(y)(x)))(\text{likes}')(\sv{\textsf{everybody}}^g)) & \text{Lexicon}%
				\\
				&{}= \sv{\textsf{somebody}}^g((\lambda {\cal Q}.\lambda x.{\cal Q}(\lambda y.\text{likes}'(y)(x)))(\sv{\textsf{everybody}}^g)) & \beta%
				\\
				&{}= \sv{\textsf{somebody}}^g(\lambda x.\sv{\textsf{everybody}}^g(\lambda y.\text{likes}'(y)(x))) & \beta%
				\\
				&{}= \sv{\textsf{somebody}}^g(\lambda x.(\lambda P.\,\text{ppl}' \subseteq \{y : P(y)\})(\lambda y.\text{likes}'(y)(x))) & \text{Lexicon}%
				\\
				&{}= \sv{\textsf{somebody}}^g(\lambda x.\,\text{ppl}' \subseteq \{y : (\lambda y.\text{likes}'(y)(x))(y)\}) & \beta%
				\\
				&{}= \sv{\textsf{somebody}}^g(\lambda x.\,\text{ppl}' \subseteq \{y : \text{likes}'(y)(x)\}) & \beta%
				\\
				&{}= (\lambda P.\,\text{ppl}' \cap \{x : P(x)\} \neq \emptyset)(\lambda x.\,\text{ppl}' \subseteq \{y : \text{likes}'(y)(x)\}) & \text{Lexicon}%
				\\
				&{}= \text{ppl}' \cap \{x : (\lambda x.\,\text{ppl}' \subseteq \{y : \text{likes}'(y)(x)\})(x)\} \neq \emptyset & \beta%
				\\
				&{}= \text{ppl}' \cap \{x : \text{ppl}' \subseteq \{y : \text{likes}'(y)(x)\}\} \neq \emptyset & \beta%
				\\
			\end{array}
		\end{array}\]
		\item In prose: there are people $x$ such that every person likes $x$.
	\end{itemize}


\section{Bonus (not required)}

\begin{itemize}
	\item A silent lexical item that allows you to assign the other interpretation to \emph{somebody likes everybody}:%	
	\[\sv{\textsf{BLA}_\emptyset^+}^g \ceq \lambda R_{\AB{e,\AB{e,t}}}.\lambda {\cal Q}_{\AB{\AB{e,t},t}}.\lambda {\cal P}_{\AB{\AB{e,t},t}}.{\cal Q}(\lambda y.{\cal P}(\lambda x.R(y)(x)))\] %
	
	Notice that this is $\eta$-equivalent to the following:
	\[\lambda R.\lambda {\cal Q}.\lambda {\cal P}.{\cal Q}(\lambda y.{\cal P}(R(y)))\] %
	
	\[\begin{array}{c}
		\begin{array}{c}
			\textsf{\Tree [.A somebody [.B [.C BLA$_\emptyset^+$ likes ] everybody ] ]}
		\end{array}
		\\\\
		\begin{array}{r@{}ll}
			\sv{\textsf{A}}^g &{}= \sv{\textsf{B}}^g(\sv{\textsf{somebody}}^g) & \bsf{FA}
			\\
			&{}= \sv{\textsf{C}}^g(\sv{\textsf{everybody}}^g)(\sv{\textsf{somebody}}^g) & \bsf{FA}%
			\\
			&{}= \sv{\textsf{BLA}_\emptyset^+}^g(\sv{\textsf{likes}}^g)(\sv{\textsf{everybody}}^g)(\sv{\textsf{somebody}}^g) & \bsf{FA}%
			\\
			&{}= (\lambda R.\lambda {\cal Q}.\lambda {\cal P}.{\cal Q}(\lambda y.{\cal P}(\lambda x.R(y)(x))))(\text{likes}')(\sv{\textsf{everybody}}^g)(\sv{\textsf{somebody}}^g) & \text{Lexicon}%
			\\
			&{}= (\lambda {\cal Q}.\lambda {\cal P}.{\cal Q}(\lambda y.{\cal P}(\lambda x.\text{likes}'(y)(x))))(\sv{\textsf{everybody}}^g)(\sv{\textsf{somebody}}^g) & \beta%
			\\
			&{}= (\lambda {\cal P}.\sv{\textsf{everybody}}^g(\lambda y.{\cal P}(\lambda x.\text{likes}'(y)(x))))(\sv{\textsf{somebody}}^g) & \beta%
			\\
			&{}= \sv{\textsf{everybody}}^g(\lambda y.\sv{\textsf{somebody}}^g(\lambda x.\text{likes}'(y)(x))) & \beta%
			\\
			&{}= \sv{\textsf{everybody}}^g(\lambda y.(\lambda P.\,\text{ppl}' \cap \{x : P(x)\} \neq \emptyset)(\lambda x.\text{likes}'(y)(x))) & \text{Lexicon}%
			\\
			&{}= \sv{\textsf{everybody}}^g(\lambda y.\,\text{ppl}' \cap \{x : (\lambda x.\text{likes}'(y)(x))(x)\} \neq \emptyset) & \beta%
			\\
			&{}= \sv{\textsf{everybody}}^g(\lambda y.\,\text{ppl}' \cap \{x : \text{likes}'(y)(x)\} \neq \emptyset) & \beta%
			\\
			&{}= (\lambda P.\,\text{ppl}' \subseteq \{y : P(y)\})(\lambda y.\,\text{ppl}' \cap \{x : \text{likes}'(y)(x)\} \neq \emptyset) & \text{Lexicon}%
			\\
			&{}= \text{ppl}' \subseteq \{y : (\lambda y.\,\text{ppl}' \cap \{x : \text{likes}'(y)(x)\} \neq \emptyset)(y)\} & \beta%
			\\
			&{}= \text{ppl}' \subseteq \{y : \text{ppl}' \cap \{x : \text{likes}'(y)(x)\} \neq \emptyset\} & \beta%
		\end{array}
	\end{array}\]

\item In prose: for every person $y$, there are people who like $y$.	
\end{itemize}


\end{document}